multiparty

theories/cgraphs/multiset.v
@@ -223,3 +223,6 @@ Proof.
   symmetry in H.
   apply multiset_op_singleton in H. eauto.
 Qed.
+
+Definition fin_multiset {A} n (f : fin n -> A) : multiset A.
+Admitted.
