theories/multiparty/invariant.v
@@ -1,0 +1,322 @@
+Require Export diris.cgraphs.genericinv.
+Require Export diris.multiparty.langdef.
+Require Export diris.multiparty.rtypesystem.
+Require Export diris.multiparty.mutil.
+
+Section bufs_typed.
+
+  Definition bufs_typed (bufs : gmap participant (gmap participant (list val)))
+                        (σs : gmap participant session_type) : rProp.
+  Admitted.
+  (* Idea: finish the proof while admitting all lemmas about bufs_typed. *)
+  (* Figure out bufs_typed later. *)
+  (* We need lemmas for preservation and a lemma for progress. *)
+  (* For progress we need that everyone receiving on empty buffers can't happen. *)
+  (* Might be able to get a tighter result: even a partial deadlock within
+     a single multiparty session cannot happen. *)
+
+  (*
+  Lemma for initialization:
+    If consistent σs then emp ⊢ bufs_typed empty_bufs σs
+
+  Lemma for close:
+    If σs is all end, then bufs_typed bufs σs ⊢ emp
+
+  Lemma for send:
+    If some type is a send, and we put something in that buffer, then it preserves bufs_typed
+
+  Lemma for receive:
+    If some type is a recv, and we take something out of that buffer, then it preserves bufs_typed
+
+  Lemma for progress:
+    If there is a buffer still allocated, then there is a participant that
+    does not have type recv and that buffer is empty.
+
+  *)
+
+    (* ∃ σs', ⌜⌜ consistent σs' ⌝⌝ ∗ big_sepM3 (λ _, buf_typed) bufs σs' σs. *)
+
+  (*
+  Global Instance bufs_typed_params : Params (@bufs_typed) 2 := {}.
+  Global Instance bufs_typed_proper b1 b2 : Proper ((≡) ==> (≡) ==> (≡)) (bufs_typed b1 b2).
+  Proof. solve_proper. Qed.
+  *)
+End bufs_typed.
+
+Section invariant.
+  Definition state_inv (es : list expr) (h : heap) (x : object) (in_l : multiset clabel) : rProp :=
+    match x with
+    | Thread n =>
+      ⌜⌜ in_l ≡ ε ⌝⌝ ∗ (* rtyped (default UnitV (es !! n)) UnitT *)
+      match es !! n with
+      | Some e => rtyped0 e UnitT
+      | None => emp
+      end
+    | Chan n => ∃ σs : gmap participant session_type,
+      ⌜⌜ in_l ≡ map_to_multiset σs ⌝⌝ ∗
+      bufs_typed (gmap_slice h n) σs
+    end%I.
+
+  Definition invariant (es : list expr) (h : heap) := inv (state_inv es h).
+End invariant.
+
+Instance state_inv_proper es h v : Proper ((≡) ==> (⊣⊢)) (state_inv es h v).
+Proof. solve_proper_prepare. destruct v; [solve_proper|by setoid_rewrite H]. Qed.
+Instance state_inv_params : Params (@state_inv) 3. Defined.
+
+
+
+Lemma bufs_typed_push (bufss : gmap participant (gmap participant (list val)))
+                      (σs : gmap participant session_type)
+                      (p q : participant) (t : type) r v :
+  σs !! p ≡ Some (SendT q t r) ->
+  val_typed v t ∗ bufs_typed bufss σs ⊢
+  bufs_typed (alter (alter (λ buf, buf ++ [v]) p) q bufss) (<[p:=r]> σs).
+Proof.
+Admitted.
+
+Lemma bufs_typed_pop (σs : gmap participant session_type)
+  (bufss : gmap participant (gmap participant (list val)))
+  (bufs : gmap participant (list val))
+  (buf : list val) (p q : participant) (v : val) (t : type) (s : session_type) :
+  σs !! p ≡ Some (RecvT q t s) ->
+  bufss !! p = Some bufs ->
+  bufs !! q = Some (v :: buf) ->
+  bufs_typed bufss σs ⊢ val_typed v t ∗
+  bufs_typed (<[ p := <[ q := buf ]> bufs ]> bufss) (<[ p := s ]> σs).
+Proof.
+Admitted.
+
+Lemma bufs_typed_dealloc bufss σs p :
+  σs !! p ≡ Some EndT ->
+  bufs_typed bufss σs ⊢
+  bufs_typed (delete p bufss) (delete p σs).
+Proof.
+Admitted.
+
+Lemma bufs_typed_empty  :
+  emp ⊢ bufs_typed ∅ ∅.
+Proof.
+Admitted.
+
+Lemma bufs_typed_empty_inv σs :
+  bufs_typed ∅ σs ⊢ ⌜⌜ σs = ∅ ⌝⌝.
+Proof.
+Admitted.
+
+Lemma init_threads_lookup (c : session) n (f : fin n -> val) (i : fin n) :
+  init_threads c n f !! fin_to_nat i =
+    Some (App (Val (f i)) (Val (ChanV (c, fin_to_nat i)))).
+Proof. Admitted.
+
+Lemma init_threads_lookup_ne (c : session) n (f : fin n -> val) (i : nat) :
+  i >= n -> init_threads c n f !! i = None.
+Proof. Admitted.
+
+Lemma gmap_slice_init_chans_ne c c' n :
+  c ≠ c' -> gmap_slice (init_chans c n) c' = ∅.
+Proof. Admitted.
+
+Lemma fin_multiset_gmap {A:ofe} n (f : fin n -> A) :
+  fin_multiset n (λ m, (fin_to_nat m, f m)) ≡ map_to_multiset (fin_gmap n f).
+Proof.
+Admitted.
+
+Lemma bufs_typed_init n i σs :
+  consistent n σs ->
+  emp ⊢ bufs_typed (gmap_slice (init_chans i n) i) (fin_gmap n σs).
+Proof.
+Admitted.
+
+Lemma preservation (threads threads' : list expr) (chans chans' : heap) :
+  step threads chans threads' chans' ->
+  invariant threads chans ->
+  invariant threads' chans'.
+Proof.
+  unfold invariant.
+  intros [i H]. destruct H.
+  destruct H as [????????HH].
+  intros Hinv.
+  destruct HH; rewrite ?right_id.
+  - (* Pure step *)
+    eapply inv_impl; last done.
+    iIntros ([] x) "H"; simpl; eauto.
+    iDestruct "H" as "[H1 H2]". iFrame.
+    rewrite list_lookup_insert_spec. case_decide; eauto.
+    destruct H2. subst. rewrite H0.
+    iDestruct (rtyped0_ctx with "H2") as (t) "[H1 H2]"; eauto.
+    iApply "H2". iApply pure_step_rtyped0; eauto.
+  - (* Send *)
+    eapply (inv_exchange (Thread i) (Chan c)); last done; try apply _.
+    + intros v x []. iIntros "H".
+      destruct v; simpl.
+      * rewrite list_lookup_insert_spec. case_decide; naive_solver.
+      * setoid_rewrite gmap_slice_alter. case_decide; naive_solver.
+    + iIntros (y0) "H". simpl. rewrite H0.
+      iDestruct "H" as (HH) "H".
+      iDestruct (rtyped0_ctx with "H") as (t) "[H1 H2]"; eauto. simpl.
+      iDestruct "H1" as (r t' ->) "[H1 H1']".
+      iDestruct "H1" as (r0 ?) "H1". simplify_eq.
+      iExists _. iFrame.
+      iIntros (x) "H". simpl in *.
+      iDestruct "H" as (σs Hσs) "H".
+      iExists (p,r).
+      rewrite list_lookup_insert; last by eapply lookup_lt_Some.
+      iSplitL "H2".
+      * iIntros "H1".
+        iSplit; eauto.
+        iApply "H2". simpl. eauto.
+      * iExists (<[ p := r ]> σs).
+        iSplit.
+        -- iPureIntro. eapply map_to_multiset_update. done.
+        -- rewrite gmap_slice_alter.
+           case_decide;simplify_eq.
+           eapply map_to_multiset_lookup in Hσs.
+           iApply bufs_typed_push; eauto with iFrame.
+  - (* Receive *)
+    eapply (inv_exchange (Thread i) (Chan c)); last done; try apply _.
+    + intros v x []. iIntros "H".
+      destruct v; simpl.
+      * rewrite list_lookup_insert_spec. case_decide; naive_solver.
+      * setoid_rewrite gmap_slice_insert. case_decide; naive_solver.
+    + iIntros (y0) "H". simpl. rewrite H0.
+      iDestruct "H" as (HH) "H".
+      iDestruct (rtyped0_ctx with "H") as (t) "[H1 H2]"; eauto. simpl.
+      iDestruct "H1" as (t' r ->) "H1".
+      iDestruct "H1" as (r0 HH') "H1". simplify_eq.
+      iExists _. iFrame.
+      iIntros (x) "H". simpl.
+      iDestruct "H" as (σs Hσs) "H".
+      iExists (p, r).
+      rewrite list_lookup_insert; last by eapply lookup_lt_Some.
+      eapply map_to_multiset_lookup in Hσs as Hp.
+      iDestruct (bufs_typed_pop with "H") as "[Hv H]"; eauto.
+      { rewrite gmap_slice_lookup //. }
+      iSplitL "H2 Hv".
+      * iIntros "H1".
+        iSplit; eauto.
+        iApply "H2". simpl.
+        iExists _,_. iSplit; first done.
+        eauto with iFrame.
+      * iExists (<[ p := r ]> σs).
+        rewrite gmap_slice_insert. case_decide; simplify_eq.
+        iFrame. iPureIntro.
+        by eapply map_to_multiset_update.
+  - (* Close *)
+    eapply (inv_dealloc (Thread i) (Chan c)); last done; try apply _.
+    + intros v x []. iIntros "H".
+      destruct v; simpl.
+      * rewrite list_lookup_insert_spec. case_decide; naive_solver.
+      * setoid_rewrite gmap_slice_delete. case_decide; naive_solver.
+    + iIntros (y0) "H". simpl. rewrite H0.
+      iDestruct "H" as (HH) "H".
+      iDestruct (rtyped0_ctx with "H") as (t) "[H1 H2]"; eauto. simpl.
+      iDestruct "H1" as (->) "H1".
+      iDestruct "H1" as (r0 HH') "H1". simplify_eq.
+      iExists _. iFrame. simpl.
+      iIntros (x) "H".
+      iDestruct "H" as (σs Hσs) "H".
+      rewrite list_lookup_insert; last by eapply lookup_lt_Some.
+      iSplitL "H2".
+      * iSplit; eauto. by iApply "H2".
+      * iExists (delete p σs).
+        iSplit.
+        -- iPureIntro. by eapply map_to_multiset_delete.
+        -- rewrite gmap_slice_delete. case_decide; simplify_eq.
+           apply map_to_multiset_lookup in Hσs.
+           by iApply bufs_typed_dealloc.
+  - (* Fork *)
+    eapply (inv_alloc_lrs (Thread i) (Chan i0)
+              n (λ i, Thread (length es + fin_to_nat i))); last done;
+      first apply _; first apply _.
+    + intros m1 m2. intro HH. simplify_eq.
+      eapply fin_to_nat_inj. lia.
+    + split_and!; eauto. intros m. split_and; eauto.
+      intros HH. simplify_eq.
+      apply lookup_lt_Some in H0. lia.
+    + intros v' x (Hn1 & Hn2 & Hn3). iIntros "H".
+      destruct v'; simpl.
+      * iDestruct "H" as "[? H]". iFrame.
+        rewrite lookup_app list_lookup_insert_spec insert_length.
+        case_decide.
+        { destruct H3. simplify_eq. }
+        destruct (es !! n0) eqn:E; eauto.
+        rewrite init_threads_lookup_ne; eauto.
+        cut (n0 - length es < n -> False); try lia.
+        intros HH.
+        specialize (Hn3 (nat_to_fin HH)). eapply Hn3.
+        f_equal. rewrite fin_to_nat_to_fin.
+        eapply lookup_ge_None in E. lia.
+      * iDestruct "H" as (σs Hσs) "H".
+        iExists σs. iSplit; eauto.
+        rewrite gmap_slice_union gmap_slice_init_chans_ne ?left_id //.
+        intros ->. simplify_eq.
+    + iIntros (x) "H". simpl.
+      iDestruct "H" as (σs Hσs) "H".
+      assert (gmap_slice h i0 = ∅) as ->.
+      {
+        eapply map_eq. intro. rewrite gmap_slice_lookup H1 lookup_empty //.
+      }
+      iDestruct (bufs_typed_empty_inv with "H") as "H".
+      iDestruct "H" as %HH.
+      iPureIntro. subst. rewrite map_to_multiset_empty in Hσs. done.
+    + iIntros (m x) "H". simpl.
+      iDestruct "H" as "[H1 H]". iFrame.
+      destruct (es !! (length es + m)) eqn:E; eauto.
+      eapply lookup_lt_Some in E. lia.
+    + iIntros (y0) "H". simpl. rewrite H0.
+      iDestruct "H" as (HH) "H".
+      iDestruct (rtyped0_ctx with "H") as (t) "[H1 H2]"; eauto. simpl.
+      iDestruct "H1" as (σs [-> Hcons]) "H1".
+      iExists (λ m, (fin_to_nat m, σs m)).
+      iSplitL "H2".
+      {
+        rewrite lookup_app list_lookup_insert; eauto using lookup_lt_Some.
+        iSplit; eauto. iApply "H2". done.
+      }
+      iSplitR.
+      {
+        iExists (fin_gmap n σs).
+        rewrite gmap_slice_union.
+        assert (gmap_slice h i0 = ∅) as ->.
+        { eapply map_eq. intro. rewrite gmap_slice_lookup lookup_empty //. }
+        rewrite right_id fin_multiset_gmap.
+        iSplit; first done.
+        iApply bufs_typed_init; eauto.
+      }
+      iApply (big_sepS_impl with "H1"). iModIntro.
+      iIntros (m _) "Ht Ho".
+      iSplit; eauto.
+      rewrite lookup_app_r. 2: { rewrite insert_length. lia. }
+      rewrite insert_length.
+      replace (length es + m - length es) with (fin_to_nat m) by lia.
+      rewrite init_threads_lookup H2.
+      simpl. eauto with iFrame.
+Qed.
+
+Lemma preservationN (threads threads' : list expr) (chans chans' : heap) :
+  steps threads chans threads' chans' ->
+  invariant threads chans ->
+  invariant threads' chans'.
+Proof. induction 1; eauto using preservation. Qed.
+
+Lemma invariant_init (e : expr) :
+  typed ∅ e UnitT -> invariant [e] ∅.
+Proof.
+  intros H.
+  eapply inv_impl; last eauto using inv_init.
+  intros. simpl. iIntros "[% H]".
+  unfold state_inv. destruct v.
+  - destruct n; simpl.
+    + subst. iSplit; eauto.
+      iApply rtyped_rtyped0_iff.
+      iApply typed_rtyped. done.
+    + subst. iFrame. eauto.
+  - iExists ∅.
+    iSplit; first done. rewrite gmap_slice_empty.
+    by iApply bufs_typed_empty.
+Qed.
+
+Lemma invariant_holds e threads chans :
+  typed ∅ e UnitT -> steps [e] ∅ threads chans -> invariant threads chans.
+Proof. eauto using invariant_init, preservationN. Qed.
