theories/multiparty/ycombinator.v
@@ -1,5 +1,5 @@
 From iris.proofmode Require Import base tactics classes.
-From diris Require Import langdef.
+From diris.multiparty Require Import langdef rtypesystem.
 
 Section ycombinator.
   (* We define the y-combinator for creating recursive functions t1 -> t2. *)
