theories/sessiontypes/invariant.v
@@ -1,7 +1,6 @@
 Require Export diris.cgraphs.genericinv.
 Require Export diris.sessiontypes.langdef.
 Require Export diris.sessiontypes.rtypesystem.
-Require Export diris.sessiontypes.langlemmas.
 
 Section bufs_typed.
   Fixpoint buf_typed (buf : list val) (ct : chan_type) (rest : chan_type) : rProp :=
